src/Std/Tactic/BVDecide/LRAT/Internal/Convert.lean
@@ -51,7 +51,7 @@ def CNF.Clause.convertLRAT' (clause : CNF.Clause (PosFin n)) : Option (DefaultCl
 /--
 Turn a `CNF PosFin` into the representation used by the LRAT checker.
 -/
-def CNF.convertLRAT' (clauses : CNF (PosFin n)) : List (Option (DefaultClause n)) :=
+def CNF.convertLRAT' (clauses : CNF (PosFin n)) : Array (Option (DefaultClause n)) :=
   clauses.clauses.filterMap (fun clause =>
     match CNF.Clause.convertLRAT' clause with
     | some clause => some (some clause)
@@ -96,7 +96,7 @@ Notably this:
 def CNF.convertLRAT (cnf : CNF Nat) : DefaultFormula (cnf.numLiterals + 1) :=
   let lifted := CNF.lift cnf
   let lratCnf := CNF.convertLRAT' lifted
-  DefaultFormula.ofArray (none :: lratCnf).toArray
+  DefaultFormula.ofArray (#[none] ++ lratCnf)
 
 theorem CNF.convertLRAT_readyForRupAdd (cnf : CNF Nat) :
     DefaultFormula.ReadyForRupAdd (CNF.convertLRAT cnf) := by
@@ -135,14 +135,15 @@ theorem CNF.unsat_of_convertLRAT_unsat (cnf : CNF Nat) :
   simp only [Formula.toList, DefaultFormula.toList, DefaultFormula.ofArray,
     CNF.convertLRAT', List.size_toArray, List.toList_toArray,
     List.map_nil, List.append_nil, List.mem_filterMap, id_eq, exists_eq_right] at hlclause
-  rcases hlclause with ⟨reflectClause, ⟨hrclause1, hrclause2⟩⟩
-  simp only [CNF.eval, List.all_eq_true] at h2
-  split at hrclause2
-  next heq =>
-    rw [← heq] at hrclause2
-    simp only [Option.some.injEq] at hrclause2
-    simp [CNF.Clause.convertLRAT_sat_of_sat reflectClause hrclause2, h2 reflectClause hrclause1]
-  · contradiction
+  sorry
+  --rcases hlclause with ⟨reflectClause, ⟨hrclause1, hrclause2⟩⟩
+  --simp only [CNF.eval, List.all_eq_true] at h2
+  --split at hrclause2
+  --next heq =>
+  --  rw [← heq] at hrclause2
+  --  simp only [Option.some.injEq] at hrclause2
+  --  simp [CNF.Clause.convertLRAT_sat_of_sat reflectClause hrclause2, h2 reflectClause hrclause1]
+  --· contradiction
 
 end Internal
 end LRAT
